fix wrong definition of 'pred_folds_perm'

viper-total-heaps/KnownFolded.thy
@@ -14,11 +14,68 @@ context begin
 private type_synonym 'a bpl_heap_ty = "ref \<times> 'a vb_field \<rightharpoonup> ('a vbpl_absval) bpl_val"
 
 
+inductive contains_heap_loc :: "heap_loc \<Rightarrow> 'a nested_mask \<Rightarrow> bool"
+  for l :: "heap_loc" where
+  ContainsLocDirect:
+  "\<lbrakk> get_mh_nm nm l > 0 \<rbrakk> \<Longrightarrow>
+   contains_heap_loc l nm"
+| ContainsLocNested:
+  "\<lbrakk> get_fnm_nm nm lp = Some (_,nm');
+     contains_heap_loc l nm' \<rbrakk> \<Longrightarrow>
+   contains_heap_loc l nm"
+
+
+lemma contains_heap_loc_stable_larger_nm:
+  assumes "contains_heap_loc l nm"
+      and "nm \<le> nm'"
+    shows "contains_heap_loc l nm'"
+  using assms
+proof (induction arbitrary: nm' rule: contains_heap_loc.inducts)
+  case (ContainsLocDirect nm)
+  then show ?case
+    by (meson KnownFolded.contains_heap_loc.ContainsLocDirect dual_order.strict_trans1 le_funE less_eq_nested_maskD)
+next
+  case (ContainsLocNested nm lp p nm')
+  show ?case
+    by (metis ContainsLocNested.IH ContainsLocNested.hyps(1) ContainsLocNested.prems Some_Some_ifD contains_heap_loc.simps nm_larger_sub_larger old.prod.inject option.inject)
+qed
+
+
+lemma contains_heap_loc_scale:
+  assumes "contains_heap_loc l nm"
+      and "s > 0"
+    shows "contains_heap_loc l (s *\<^sub>s nm)"
+  using assms(1)
+proof (induction rule: contains_heap_loc.inducts)
+  case (ContainsLocDirect nm)
+  show ?case
+    apply (rule contains_heap_loc.ContainsLocDirect)
+    using ContainsLocDirect
+    apply (cases nm)
+    unfolding scale_nested_mask_def
+    apply (simp add: mul_mask_def)
+    using assms(2) preal_to_real(2,7,9)
+    by auto
+next
+  case (ContainsLocNested nm lp p' nm')
+  have "get_fnm_nm (s *\<^sub>s nm) lp = Some ((Abs_posreal s) * p', s *\<^sub>s nm')"
+    using ContainsLocNested.hyps(1)
+    unfolding scale_nested_mask_def
+    apply (cases nm)
+    apply simp
+    using assms(2) mult.commute
+    by blast
+  show ?case
+    apply (rule contains_heap_loc.ContainsLocNested)
+    by fact+
+qed
+
+
 inductive pred_folds_perm :: "'a predicate_loc \<Rightarrow> heap_loc \<Rightarrow> 'a nested_mask \<Rightarrow> bool"
   for lp :: "'a predicate_loc" and l :: "heap_loc" where
   ContainsPermDirect:
   "\<lbrakk> get_fnm_nm nm lp = Some (_,nm');
-     get_mh_nm nm' l > 0 \<rbrakk> \<Longrightarrow>
+     contains_heap_loc l nm' \<rbrakk> \<Longrightarrow>
    pred_folds_perm lp l nm"
 | ContainsPermNested:
   "\<lbrakk> get_fnm_nm nm lp' = Some (_,nm');
@@ -44,22 +101,20 @@ lemma pred_folds_perm_stable_larger_nm:
   using assms
 proof (induction arbitrary: nm' rule: pred_folds_perm.inducts)
   case (ContainsPermDirect nm p nm_sub)
-  obtain p' nm_sub' where "get_fnm_nm nm' lp = Some (p', nm_sub')" and "nm_sub \<le> nm_sub'"
-    apply (cases nm; cases nm')
-    using ContainsPermDirect.prems[unfolded less_eq_nested_mask_def]
-    apply simp
-    by (smt (verit, del_insts) ContainsPermDirect.hyps(1) get_fnm_nm.simps has_Some_iff less_eq_nested_mask_def option_fold.simps(1) order_le_less prod.exhaust_sel snd_conv)
+  then obtain p' nm_sub' where "get_fnm_nm nm' lp = Some (p', nm_sub')" and "nm_sub \<le> nm_sub'"
+    using nm_larger_sub_larger_not_None
+    by blast
   show ?case
     apply (rule pred_folds_perm.ContainsPermDirect)
      apply fact
-    by (meson ContainsPermDirect.hyps(2) \<open>nm_sub \<le> nm_sub'\<close> dual_order.strict_trans1 le_funE less_eq_nested_maskD)
+    by (meson ContainsPermDirect.hyps(2) \<open>nm_sub \<le> nm_sub'\<close> contains_heap_loc_stable_larger_nm)
 next
   case (ContainsPermNested nm lp' p nm_sub)
   obtain mh fnm where "nm = NM mh fnm" using nm_get_eq by blast
   obtain mh' fnm' where "nm' = NM mh' fnm'" using nm_get_eq by blast
   obtain p' nm_sub' where "get_fnm_nm nm' lp' = Some (p', nm_sub')" and "nm_sub \<le> nm_sub'"
-    using ContainsPermNested.prems[unfolded less_eq_nested_mask_def \<open>nm = _\<close> \<open>nm' = _\<close>, simplified]
-    by (smt (verit) ContainsPermNested.hyps(1) \<open>nm = NM mh fnm\<close> \<open>nm' = NM mh' fnm'\<close> get_fnm_nm.simps has_Some_iff less_eq_nested_mask_def option_fold.simps(1) order_le_less prod.exhaust_sel snd_conv)
+    using nm_larger_sub_larger_not_None ContainsPermNested.hyps(1) ContainsPermNested.prems
+    by blast
   show ?case
     apply (rule pred_folds_perm.ContainsPermNested)
      apply fact
@@ -70,8 +125,8 @@ qed
 lemma pred_folds_perm_plus_l:
   assumes "pred_folds_perm lp l nm"
     shows "pred_folds_perm lp l (nm' + nm)"
-  using assms nested_mask_greater_equiv pred_folds_perm_stable_larger_nm add.commute
-  by blast
+  apply (rule pred_folds_perm_stable_larger_nm[OF assms(1)])
+  by (simp add: add.commute nm_sum_is_bigger)
 
 
 lemma pred_folds_perm_plus_r:
@@ -94,10 +149,7 @@ proof (induction rule: pred_folds_perm.inducts)
      apply (simp add: scale_nested_mask_def)
     using ContainsPermDirect.hyps(1) assms(2) mult.commute
      apply auto[1]
-    apply (cases nm')
-    apply (simp add: scale_nested_mask_def mul_mask_def)
-    using ContainsPermDirect.hyps(2) assms(2) preal_to_real(2,7,9)
-    by auto
+    by (simp add: ContainsPermDirect.hyps(2) assms(2) contains_heap_loc_scale)
 next
   case (ContainsPermNested nm lp' p nm')
   show ?case
